x86/Asm.v
@@ -321,7 +321,7 @@ Open Scope asm.
 Fixpoint undef_regs (l: list preg) (rs: regset) : regset :=
   match l with
   | nil => rs
-  | r :: l' => undef_regs l' (rs#r <- Vundef)
+  | r :: l' => undef_regs l' rs#r <- Vundef
   end.
 
 (** Assigning a register pair *)
@@ -1183,7 +1183,7 @@ Inductive step {exec_load exec_store} `{!MemAccessors exec_load exec_store} (ge:
         (RA_NOT_VUNDEF: rs RA <> Vundef)
       ,      (* CompCertX: END additional conditions for calling convention *)
         external_call ef ge args m t res m' ->
-        rs' = (set_pair (loc_external_result (ef_sig ef)) res rs) #PC <- (rs RA) #RA <- Vundef ->
+        rs' = (set_pair (loc_external_result (ef_sig ef)) res (undef_regs (CR ZF :: CR CF :: CR PF :: CR SF :: CR OF :: nil) (undef_regs (map preg_of destroyed_at_call) rs))) #PC <- (rs RA) #RA <- Vundef ->
         step ge (State rs m) t (State rs' m').
 
 End RELSEM.
